---
id: doc1
title: Perfect Square Formula
sidebar_label: Perfect Square Formula
---

Click [here](https://docusaurus.io) to access Mathium's perfect square formula calculator.

## Intro

When any polynomial is multiplied by itself, then it is a perfect square.

To expand any polynomial, we can apply one of the following patterns: 



```
(a + b)^2 = a^2 + 2ab + b^2

(a - b)^2 = a^2 - 2ab - b^2
```

NOTE: In these patterns, ```a``` and/or ```b``` can be replaced by any type of algebraic expression.

For example, if we want to expand ```(8x + 7x)^2```, ```a = 8x``` and ```b = 7x```. Therefore...

```
(8x + 7x)^2 = (8x)^2 + 2(8x)(7x) + (7x)^2
```

## Example 1: (2x + 8)^2

Suppose we are given the expression ```(2x + 8)^2```.

When applying the Perfect Square Formula, the result would be the following:

```
(2x + 8)^2 = (2x)^2 + 2(2x)(8) + (8)^2
```
## Example 2: (7 + 9)^2

Suppose we are given the expression ```(7 + 9)^2```.

When applying the Perfect Square Formula, the result would be the following:

```
(7 + 9)^2 = (7)^2 + 2(7)(9) + (9)^2

= 49 + 126 + 81

= 256
```
## Example 3: (98x + 54y)^2

Suppose we are given the expression ```(98x + 54y)^2```.

When applying the Perfect Square Formula, the result would be the following:

```
(98x + 54y)^2 = (98x)^2 + 2(98x)(54y) + (54y)^2
```

